@prefix cms: <http://mu.semte.ch/vocabulary/cms/>.
@prefix adres: <http://data.vlaanderen.be/ns/adres#>.
@prefix skos: <http://www.w3.org/2004/02/skos/core#>.
@prefix locn: <http://www.w3.org/ns/locn#>.
@prefix dct: <http://purl.org/dc/terms/>.
@prefix prov: <http://www.w3.org/ns/prov#>.
@prefix cidoc: <http://www.cidoc-crm.org/cidoc-crm/>.
@prefix ext: <http://mu.semte.ch/vocabularies/ext/>.
@prefix rm: <http://mu.semte.ch/vocabularies/logical-delete/>.
@prefix typedLiterals: <http://mu.semte.ch/vocabularies/typed-literals/>.
@prefix mu: <http://mu.semte.ch/vocabularies/core/>.
@prefix xsd: <http://www.w3.org/2001/XMLSchema#>.
@prefix app: <http://mu.semte.ch/app/>.
@prefix owl: <http://www.w3.org/2002/07/owl#>.
@prefix rdf: <http://www.w3.org/1999/02/22-rdf-syntax-ns#>.
@prefix dc: <http://purl.org/dc/elements/1.1/>.

<http://mu.semte.ch/ontology> rdf:type owl:Ontology.
<http://mu.semte.ch/ontology> dc:title "Generated resource ontology". 
<http://mu.semte.ch/ontology> dc:description "Generated resource ontology". 

cidoc:E22_Man-Made_Object rdf:type owl:Class;
  rdfs:label "aanduidingsobject".
locn:Address rdf:type owl:Class;
   rdfs:subClassOf prov:Location;
  rdfs:label "address".
prov:Location rdf:type owl:Class;
  rdfs:label "location".
besluit:Besluit rdf:type owl:Class;
  rdfs:label "besluit".
skos:Concept rdf:type owl:Class;
  rdfs:label "typology".

cidoc:P102_has_title rdf:type owl:DatatypeProperty;
  rdfs:comment "Resources type is string.  Original predicate is cidoc:P102_has_title.";
  rdfs:label "title";
  rdfs:range rdfs:Literal;
  rdfs:domain cidoc:E22_Man-Made_Object.
cidoc:P3_has_note rdf:type owl:DatatypeProperty;
  rdfs:comment "Resources type is string.  Original predicate is cidoc:P3_has_note.";
  rdfs:label "description";
  rdfs:range rdfs:Literal;
  rdfs:domain cidoc:E22_Man-Made_Object.
dct:identifier rdf:type owl:DatatypeProperty;
  rdfs:comment "Resources type is string.  Original predicate is dct:identifier.";
  rdfs:label "identifier";
  rdfs:range rdfs:Literal;
  rdfs:domain cidoc:E22_Man-Made_Object.
ext:artStyle rdf:type owl:DatatypeProperty;
  rdfs:comment "Resources type is string.  Original predicate is ext:artStyle.";
  rdfs:label "style";
  rdfs:range rdfs:Literal;
  rdfs:domain cidoc:E22_Man-Made_Object.
dct:created rdf:type owl:DatatypeProperty;
  rdfs:comment "Resources type is datetime.  Original predicate is dct:created.";
  rdfs:label "creation";
  rdfs:range rdfs:Literal;
  rdfs:domain cidoc:E22_Man-Made_Object.
dct:modified rdf:type owl:DatatypeProperty;
  rdfs:comment "Resources type is datetime.  Original predicate is dct:modified.";
  rdfs:label "location";
  rdfs:range rdfs:Literal;
  rdfs:domain cidoc:E22_Man-Made_Object.
adres:gemeentenaam rdf:type owl:DatatypeProperty;
  rdfs:comment "Resources type is string.  Original predicate is adres:gemeentenaam.";
  rdfs:label "municipality-name";
  rdfs:range rdfs:Literal;
  rdfs:domain locn:Address.
locn:adminUnitL2 rdf:type owl:DatatypeProperty;
  rdfs:comment "Resources type is string.  Original predicate is locn:adminUnitL2.";
  rdfs:label "province";
  rdfs:range rdfs:Literal;
  rdfs:domain locn:Address.
locn:thoroughfare rdf:type owl:DatatypeProperty;
  rdfs:comment "Resources type is string.  Original predicate is locn:thoroughfare.";
  rdfs:label "street-name";
  rdfs:range rdfs:Literal;
  rdfs:domain locn:Address.
locn:postCode rdf:type owl:DatatypeProperty;
  rdfs:comment "Resources type is string.  Original predicate is locn:postCode.";
  rdfs:label "postal-code";
  rdfs:range rdfs:Literal;
  rdfs:domain locn:Address.
adres:Adresvoorstelling.busnummer rdf:type owl:DatatypeProperty;
  rdfs:comment "Resources type is string.  Original predicate is adres:Adresvoorstelling.busnummer.";
  rdfs:label "bus-number";
  rdfs:range rdfs:Literal;
  rdfs:domain locn:Address.
dct:title rdf:type owl:DatatypeProperty;
  rdfs:comment "Resources type is string.  Original predicate is dct:title.";
  rdfs:label "title";
  rdfs:range rdfs:Literal;
  rdfs:domain besluit:Besluit.
skos:prefLabel rdf:type owl:DatatypeProperty;
  rdfs:comment "Resources type is string.  Original predicate is skos:prefLabel.";
  rdfs:label "title";
  rdfs:range rdfs:Literal;
  rdfs:domain skos:Concept.


cidoc:P53_has_former_or_current_location rdf:type owl:ObjectProperty;
  rdfs:comment "";
  rdfs:label "address";
  rdfs:domain cidoc:E22_Man-Made_Object;
  rdfs:range locn:Address.
cidoc:P2_has_type rdf:type owl:ObjectProperty;
  rdfs:comment "";
  rdfs:label "typology";
  rdfs:domain cidoc:E22_Man-Made_Object;
  rdfs:range skos:Concept.



